feat: restriction of permutation

Fifteen/Data/Array/Basic.lean
@@ -16,7 +16,7 @@ import Fifteen.Data.List.Basic
 -- Disable auto-binding of unbounded variables
 set_option autoImplicit false
 
-universe u v
+universe u v w
 
 namespace Array
 
@@ -29,6 +29,22 @@ This theorem depends on `Classical.choice` since `Array.append_data` does.
 -/
 theorem size_append (as bs : Array α) : (as ++ bs).size = as.size + bs.size := by
   dsimp [size]; rw [append_data, List.length_append]
+
+theorem size_shrink_loop (as : Array α) {k : Nat} (h : k ≤ as.size) : (shrink.loop k as).size = as.size - k := by
+  induction k generalizing as with
+  | zero => rfl
+  | succ k IH =>
+    dsimp [shrink.loop]
+    have : as.size = as.pop.size + 1 := by
+      rw [as.size_pop, Nat.sub_add_cancel (trans (r:=LE.le (α:=Nat)) (s:=LT.lt (α:=Nat)) k.zero_le h)]
+    rewrite [this] at h ⊢
+    rewrite [IH as.pop (Nat.le_of_succ_le_succ h)]
+    simp only [Nat.succ_sub_succ_eq_sub]
+
+theorem size_shrink (as : Array α) {n : Nat} (h : n ≤ as.size) : (as.shrink n).size = n := by
+  refine Eq.trans (size_shrink_loop as ?_) ?_
+  . exact as.size.sub_le_self n
+  . exact Nat.sub_sub_self h
 
 theorem any_eq_any_data (as : Array α) (p : α → Bool) : as.any p = as.data.any p := by
   dsimp [any, anyM]; simp
@@ -58,7 +74,70 @@ theorem swap_comm (as : Array α) (i j : Fin as.size) : as.swap i j = as.swap j 
     rw [List.set_comm _ _ _ h]
 
 
+/-! ### Declarations about `Array.pam` -/
+
+section PMap
+
+variable {β : Type v} {p : α → Prop}
+/--
+The runtime implementation of `Array.pmapM`.
+This function is just an alias of `Array.mapMUnsafe`.
+-/
+@[inline]
+unsafe def pmapMUnsafe {m : Type v → Type w} [Monad m] (f : (a : α) → p a → m β) (as : Array α) (_ : ∀ (i : Nat) (hi : i < as.size), p as[i]) : m (Array β) :=
+  as.mapMUnsafe fun a => f a lcProof
+
+/-- The `Array`-counterpart of `List.pmap` in a monad context. -/
+@[implemented_by pmapMUnsafe]
+def pmapM {m : Type v → Type w} [Monad m] (f : (a : α) → p a → m β) (as : Array α) (h : ∀ (i : Nat) (hi : i < as.size), p as[i]) : m (Array β) :=
+  let rec map (i : Nat) (r : Array β) : m (Array β) := do
+    if hlt : i < as.size then
+      map (i+1) (r.push (← f as[i] (h i hlt)))
+    else
+      pure r
+  map 0 (Array.mkEmpty as.size)
+termination_by map => as.size - i
+
+/-- The `Array`-counterpart of `List.pmap`. -/
+@[inline]
+def pmap (f : (a : α) → p a → β) (as : Array α) (h : ∀ (i : Nat) (hi : i < as.size), p as[i]) : Array β :=
+  pmapM (m:=Id) f as h
+
+theorem pmap_eq_nat_fold'_push (f : (a : α) → p a → β) (as : Array α) (h : ∀ (i : Nat) (hi : i < as.size), p as[i]) : as.pmap f h = Nat.fold' as.size (fun i x => x.push <| f as[i.1] (h i.1 i.2)) #[] := by
+  rewrite [Nat.fold'_eq_fold'TR]
+  dsimp [pmap, pmapM, Nat.fold'TR]
+  suffices ∀ (k : Nat) (hk : k ≤ as.size) (bs : Array β), pmapM.map (m:=Id) f as h (as.size - k) bs = Nat.fold'TR.loop as.size _ k hk bs
+  from Eq.trans (as.size.sub_self ▸ rfl) (this as.size .refl #[])
+  intro k hk bs
+  induction k generalizing bs with
+  | zero =>
+    simp only [Nat.zero_eq, Nat.sub_zero]
+    unfold pmapM.map
+    exact dif_neg <| Nat.lt_irrefl as.size
+  | succ k IH =>
+    unfold pmapM.map
+    rewrite [dif_pos (trans (as.size.sub_succ_lt_self _ hk) (as.size.sub_le k))]
+    dsimp [Nat.fold'TR.loop]
+    rw [← IH (Nat.le_of_succ_le hk) _]
+    apply congrFun; apply congrArg
+    rewrite [← Nat.sub_add_comm hk]
+    exact Nat.succ_sub_succ_eq_sub as.size k
+
+theorem size_pmap (f : (a : α) → p a → β) (as : Array α) (h : ∀ (i : Nat) (hi : i < as.size), p as[i]) : (as.pmap f h).size = as.size := by
+  rewrite [pmap_eq_nat_fold'_push]
+  refine Nat.fold'_induction (motive := fun k (x : Array β) => x.size = k) as.size _ #[] rfl ?_
+  intro i hi x hx
+  simp only [size_push, hx]
+
+end PMap
+
+
 /-! ### Lemmas about `GetElem.getElem` -/
+
+theorem getElem_pop (as : Array α) (i : Nat) (hi : i < as.pop.size) : as.pop[i] = as[i]'(trans (r:=LT.lt (α:=Nat)) (s:=LE.le) hi (as.size_pop ▸ as.size.sub_le_self 1)) := by
+  dsimp [pop]
+  simp only [getElem_eq_data_get, List.dropLast_eq_take, List.get_take]
+  exact as.data.get_take _ i
 
 theorem getElem_swap (as : Array α) (i j : Fin as.size) (k : Nat) {hk : k < (as.swap i j).size} : (as.swap i j)[k] = if j.1 = k then as[i.1] else if i.1 = k then as[j.1] else as[k]'(as.size_swap i j ▸ hk) := by
   have : ∀ {m n : Nat} (h : m = n) (i : Fin m), ((h ▸ i) : Fin n).val = i.val :=
@@ -87,6 +166,43 @@ theorem getElem_append_right {i : Nat} (as bs : Array α) (h : i ≥ as.size) {h
   rewrite [List.get_of_eq (Array.append_data as bs)]
   rewrite [List.get_append_right' h]
   rfl
+
+theorem getElem_shrink (as : Array α) {n : Nat} (h : n ≤ as.size) (i : Nat) (hi : i < (as.shrink n).size) : (as.shrink n)[i] = as[i]'(trans (r:=LT.lt (α:=Nat)) (as.size_shrink h ▸ hi) h) := by
+  dsimp [shrink] at hi ⊢
+  revert i
+  suffices ∀ (i k : Nat) (hk : k ≤ as.size) (hi : i < as.size - k), (shrink.loop k as)[i]'(as.size_shrink_loop hk ▸ hi) = as[i]'(trans (r:=LT.lt (α:=Nat)) hi (as.size.sub_le_self k))
+  from fun i hi =>
+    this i (as.size - n) (as.size.sub_le_self n) (by rw [Nat.sub_sub_self h]; exact trans (r:=LT.lt (α:=Nat)) (s:=Eq) hi (as.size_shrink h))
+  clear h n
+  intro i k hk hi
+  induction k generalizing as with
+  | zero => rfl
+  | succ k IH =>
+    dsimp [shrink.loop]
+    specialize IH as.pop (as.size_pop ▸ Nat.le_sub_of_add_le hk) (by rewrite [as.size_pop, Nat.sub_sub, Nat.add_comm]; exact hi)
+    rewrite [IH]
+    exact as.getElem_pop i _
+
+/--
+:::note warn
+This lemma depends on `Classical.choice` because of `Array.get_push_eq` and `Array.get_push_lt`.
+:::
+-/
+theorem getElem_pmap {β : Type v} {p : α → Prop} (f : (a : α) → p a → β) (as : Array α) (h : ∀ (i : Nat) (hi : i < as.size), p as[i]) (i : Nat) {hi : i < (as.pmap f h).size} : (as.pmap f h)[i] = f (as[i]'(as.size_pmap f h ▸ hi)) (h i <| as.size_pmap f h ▸ hi) := by
+  simp only [pmap_eq_nat_fold'_push]
+  refine Nat.fold'_induction
+    (motive := fun (k : Nat) (bs : Array β) => ∀ (j : Nat) (hjk : j < k) (hk : k ≤ as.size) (hbsk : bs.size = k), bs[j]'(hbsk ▸ hjk) = f (as[j]'(trans (r:=LT.lt (α:=Nat)) hjk hk)) (h j (trans (r:=LT.lt (α:=Nat)) hjk hk)))
+    as.size _ #[] ?_ ?_ i (as.size_pmap f h ▸ hi) .refl ((as.pmap_eq_nat_fold'_push f h) ▸ as.size_pmap f h)
+  . intro k hk; cases hk
+  . intro k hk bs IH j hj _ hbsk
+    simp only [Array.size_push] at hbsk ⊢
+    cases hbsk
+    cases Nat.eq_or_lt_of_le (Nat.le_of_succ_le_succ hj) with
+    | inl heq =>
+      cases heq; exact get_push_eq ..
+    | inr hlt =>
+      rewrite [bs.get_push_lt _ j hlt]
+      exact IH j hlt (Nat.le_of_lt hk) rfl
 
 
 /-! ### Membership relation -/
