Fifteen/Data/Nat/Basic.lean
@@ -4,6 +4,7 @@ Released under Apache 2.0 license as described in the file LICENSE.
 -/
 
 import Std.Data.Nat.Lemmas
+import Std.Data.Fin.Basic
 
 /-!
 # Auxiliary declarations about `Nat`
@@ -16,6 +17,9 @@ universe u v
 
 
 namespace Nat
+
+theorem sub_le_self (m n : Nat) : m - n ≤ m :=
+  sub_le_of_le_add <| m.le_add_right n
 
 @[elab_as_elim]
 theorem decreasing_induction {motive : Nat → Prop} (succ : ∀ n, motive (n+1) → motive n) {m n : Nat} (beg : motive n) (h : m ≤ n) : motive m := by
@@ -35,6 +39,21 @@ def dfold {α : Nat → Sort u} (f : (n : Nat) → α n → α (n+1)) (n : Nat) 
   match n with
   | 0 => init
   | n+1 => f n (dfold f n init)
+
+theorem dfold_congr {α β : Nat → Sort u} {f : (n : Nat) → α n → α (n+1)} {g : (n : Nat) → β n → β (n+1)} (hfg : ∀ n a b, HEq a b → HEq (f n a) (g n b)) (n : Nat) {a : α 0} {b : β 0} (hab : HEq a b) : HEq (dfold f n a) (dfold g n b) := by
+  have : α = β := funext fun n => by
+    suffices ∃ (a : α n) (b : β n), HEq a b
+    from let ⟨_,_,hab⟩ := this; type_eq_of_heq hab
+    induction n with
+    | zero => exact ⟨a,b,hab⟩
+    | succ n IH =>
+      let ⟨a,b,hab⟩ := IH
+      exact ⟨f n a, g n b, hfg n a b hab⟩
+  cases this; cases hab
+  simp only [heq_iff_eq] at hfg ⊢
+  induction n with
+  | zero => rfl
+  | succ n IH => dsimp [dfold]; exact hfg n _ _ IH
 
 /--
 Induction principle on the value computed by `Nat.dfold`.
@@ -68,6 +87,31 @@ def fold' {α : Type u} (n : Nat) (f : Fin n → α → α) (init : α) : α :=
   dfold (α := fun i => i ≤ n → α)
     (fun i x hi => f ⟨i,hi⟩ (x <| Nat.le_of_lt hi))
     n (fun _ => init) .refl
+
+theorem fold'_congr {α : Type u} {m n : Nat} (h : m = n) {f : Fin m → α → α} {g : Fin n → α → α} (hf : ∀ i j a, i.1 = j.1 → f i a = g j a) (init : α) : fold' m f init = fold' n g init := by
+  cases h
+  have : f = g := funext fun i => funext fun a =>
+    hf i i a rfl
+  cases this
+  rfl
+
+@[simp]
+theorem fold'_zero {α : Type u} (f : Fin 0 → α → α) (init : α) : fold' 0 f init = init :=
+  rfl
+
+theorem fold'_succ {α : Type u} (n : Nat) (f : Fin (n+1) → α → α) (init : α) : fold' (n+1) f init = f (Fin.last n) (fold' n (f ∘ Fin.castSucc) init) := by
+  dsimp [fold', dfold]
+  apply congrArg
+  let mot₁ : Nat → Type u := fun i => i ≤ n+1 → α
+  let mot₂ : Nat → Type u := fun i => i ≤ n → α
+  suffices ∀ (k : Nat) (hk : k ≤ n), dfold (α:=mot₁) _ k (fun _ => init) (.step hk) = dfold (α:=mot₂) _ k (fun _ => init) hk
+  from this n .refl
+  intro k hk
+  induction k with
+  | zero => rfl
+  | succ k IH =>
+    dsimp [dfold]; apply congrArg
+    exact IH (Nat.le_of_succ_le hk)
 
 /--
 Induction principle on the computation of `Nat.fold'`.
@@ -103,5 +147,38 @@ theorem fold'_hom
   intro k
   refine dfold_hom f' g₁' g₂' k init' ?_
   intro i x; dsimp; simp only [H]
+
+@[inline]
+def fold'TR {α : Type u} (n : Nat) (f : Fin n → α → α) (init : α) : α :=
+  let rec @[specialize] loop : (k : Nat) → k ≤ n → α → α
+  | 0  , _, a => a
+  | k+1, hk, a =>
+    let i : Fin n := .mk (n - (k+1)) <|
+      Nat.sub_lt_of_pos_le k.zero_lt_succ hk
+    loop k (Nat.le_of_succ_le hk) <| f i a
+  loop n .refl init
+
+@[csimp]
+theorem fold'_eq_fold'TR : @fold' = @fold'TR := by
+  funext α n f init
+  suffices ∀ (m n k : Nat) (h : m + n = k) (f : Fin k → α → α), fold'TR.loop k f m (h ▸ m.le_add_right n) (fold' n (fun i => f ⟨i.1, trans i.2 (h ▸ n.le_add_left m)⟩) init) = fold' k f init
+  from (this n 0 _ rfl f).symm
+  clear n f
+  intro m n k h f
+  induction m generalizing n k init with
+  | zero =>
+    rewrite [zero_eq, Nat.zero_add] at h; cases h
+    simp only [fold'TR.loop, zero_eq]
+  | succ m IH =>
+    rewrite [Nat.succ_add] at h; cases h
+    dsimp [fold'TR.loop]
+    have := fun a => IH a (n+1) (m+n+1) rfl f
+    conv at this =>
+      ext a; lhs; arg 5; rewrite [fold'_succ]
+    rewrite [← this init]
+    apply congrArg; apply congrFun; apply congrArg
+    apply Fin.eq_of_val_eq
+    simp only [Nat.succ_sub_succ_eq_sub, Nat.add_sub_cancel_left]
+    rfl
 
 end Nat
